added parsing verification

dnsprotect/cleanup/DNSprotect4.dfy
@@ -13,6 +13,16 @@ study.
 
 
 
+
+
+
+
+
+
+
+
+
+
 include "lucidBase4.dfy"
 
 
@@ -36,13 +46,101 @@ include "lucidBase4.dfy"
 
 
 
-module LucidProg refines LucidBase { 
-      import opened Memop
-      
-      type counter = uint32              // limit must exceed U
 
-      datatype Event =
+
+
+
+
+
+
+
+
+
+
+
+
+
+module LucidProg refines LucidBase { 
+   import opened Memop
+
+   // Parser
+   ghost predicate valid_parser_input(p:Pkt) 
+   {
+      |p.bytes| > 44  // 14 (eth) + 20 (ipv4) + 8 (udp) + 2 (dns request id)
+   }
+
+   ghost predicate parser_spec(p : Pkt, d : ParseDecision<Event>) 
+   {
+      if (p.bytes[12] != 0x08 || p.bytes[13] != 00) then d.GenerateExtern?  // non-ipv4 are dropped
+      else if (p.bytes[23] != 0x11) then d.GenerateExtern?                  // non-udp are dropped
+      else if ((cast_int16(p.bytes[34..36]) == 53))               // sport == 53 => response
+         then (
+            match d 
+               case Generate(ProcessPacket(false, _)) => true
+               case _ => false
+         )
+      else if ((cast_int16(p.bytes[36..38]) == 53))               // dport == 53 => request
+         then (
+            match d 
+               case Generate(ProcessPacket(true, _)) => true
+               case _ => false
+         )
+      else d.GenerateExtern?                               // neither sport nor dport == 53 => forward 
+   }
+
+   function parse(p : Pkt) : ParseDecision<Event>  
+   { 
+    ghost var pre_eth := p.bytes;
+    var (p, dmac) := read48(p);
+    // int<48> dmac = read(48, p);
+    var (p, smac) := read48(p);
+    var (p, ethType) := read16(p);
+    if (ethType == 0x0800) then
+        var p := skip(p, 9);// skip to proto
+        var (p, proto) := read8(p);
+        if (proto == 0x11) then 
+            var p := skip(p, 10); // skip to udp
+            ghost var pre_sport := p.bytes;
+            var (p, sport) := read16(p);
+            ghost var pre_dport := p.bytes;
+            var (p, dport) := read16(p);
+
+            assert (pre_sport[0..2] == pre_eth[34..36]);
+            assert (pre_dport[0..2] == pre_eth[36..38]);
+
+            match (sport, dport) 
+            case (53, _) =>             // case: dns response
+                assert (cast_int16(pre_sport[0..2]) == 53);
+                var dnsRequest := false;
+                var p := skip(p, 4); // skip to dns
+                var (p, dnsId) := read16(p);
+                Generate(ProcessPacket(dnsRequest, dnsId))
+            case (_, 53) =>               // case dns request
+                assert (cast_int16(pre_sport[0..2]) != 53);
+                assert (cast_int16(pre_dport[0..2]) == 53);
+                var dnsRequest := true;
+                var p := skip(p, 4); // skip to dns
+                var (p, dnsId) := read16(p);
+                Generate(ProcessPacket(dnsRequest, dnsId))
+            case (_, _) =>                   // case: non-dns
+                assert (cast_int16(pre_sport[0..2]) != 53);
+                assert (cast_int16(pre_dport[0..2]) != 53);
+               //  assert (pre_sport[0..2] == pre_eth[34..36]);
+               //  assert (pre_dport[0..2] == pre_eth[36..38]);
+                assert (cast_int16(pre_eth[34..36]) != 53);
+                assert (cast_int16(pre_eth[36..38]) != 53);
+                GenerateExtern("Forward")
+        else 
+            GenerateExtern("Forward")      // not udp: forward
+    else // not ipv4 -- drop
+        GenerateExtern("Forward")         // not ipv4: forward
+   }
+      
+   type counter = uint32              // limit must exceed U
+
+   datatype Event =
       | ProcessPacket (dnsRequest: bool, uniqueSig: uint16)
+      | ForwardPacket()
       | SimulatedClockTick ()
       | SimulatedHardwareFailure () 
       | SetFiltering (toWhat: bool)
@@ -134,6 +232,7 @@ module LucidProg refines LucidBase {
                case e.SimulatedHardwareFailure? => 
                   simulatedHardwareFailure ();
                case e.Non? => 
+               case e.ForwardPacket? => 
             }
          } 
 
@@ -177,7 +276,7 @@ module LucidProg refines LucidBase {
                generate_port(1, ProcessPacket(false, uniqueSig)); 
             }
          }   
-      }
+      } 
 
       method processRequest (uniqueSig: uint16)
          modifies this
